x86/Reloctablesgenproof.v
@@ -1,0 +1,52 @@
+(* *******************  *)
+(* Author: Pierre Wilke *)
+(* Date:   Jan 30, 2020 *)
+(* *******************  *)
+
+Require Import Coqlib Errors.
+Require Import Integers Floats AST Linking.
+Require Import Values Memory Events Globalenvs Smallstep.
+Require Import Op Locations Mach Conventions Asm RealAsm.
+Require Import RelocProgram RelocProgSemantics RelocProgSemantics1.
+Require Import Reloctablesgen.
+Import ListNotations.
+
+Definition match_prog p tp :=
+  transf_program p = OK tp.
+
+Lemma transf_program_match:
+  forall p tp, transf_program p = OK tp -> match_prog p tp.
+Proof.
+  unfold match_prog; intuition.
+Qed.
+
+Section PRESERVATION.
+  Existing Instance inject_perm_all.
+Context `{external_calls_prf: ExternalCalls}.
+
+Local Existing Instance mem_accessors_default.
+
+
+Variables prog tprog: RelocProgram.program.
+
+Hypothesis TRANSF: match_prog prog tprog.
+
+Lemma transf_program_correct:
+  forall rs, forward_simulation (RelocProgSemantics.semantics prog rs)
+                                (RelocProgSemantics1.semantics tprog rs).
+Proof.
+Admitted.
+
+End PRESERVATION.
+
+Require Import RelocLinking.
+
+Instance reloctablesgen_linker : Linker RelocProgram.program.
+Admitted.
+
+Instance reloctablesgen_transflink : @TransfLink _ _ RelocLinking.Linker_reloc_prog reloctablesgen_linker match_prog.
+Proof.
+  red. simpl.
+  unfold match_prog.
+  intros. simpl.
+Admitted.
